
Because we want the list in **ascending** order, we simply work backwards starting at the last index's (m - 1,  n - 1,  m + n - 1). That way, when the code finishes executing, the newly merged array will be in ascending order as we are adding them to the **end** of nums1 (the merged array) at p (**the end index of nums1**).

### Code Example:

```python
class Solution(object):

    def merge(self, nums1, m, nums2, n):

        """

        :type nums1: List[int]

        :type m: int

        :type nums2: List[int]

        :type n: int

        :rtype: None Do not return anything, modify nums1 in-place instead.

        """

        p1 = m - 1

        p2 = n - 1

        p = m + n - 1 # combined length

  

        while p1 >= 0 and p2 >= 0:

            if nums1[p1] > nums2[p2]: # if the value at p1 (nums1) is smaller than p2 (nums2)

                nums1[p] = nums1[p1] # add p1 to the nums array

                p1 -= 1 # move to the next value in nums1

            else:

                nums1[p] = nums2[p2] # else add the value in nums2 to nums 1

                p2 -= 1 # move to next value in nums2

            p -= 1 # move to next value in nums1

  

        while p2 >= 0: # add any remaining values

            nums1[p] = nums2[p2]

            p -= 1

            p2 -= 1
```